tutorial/utp_csp_buffer.thy
@@ -29,15 +29,19 @@ type_synonym act_buffer = "(st_buffer, ch_buffer) action"
 text \<open> We define an action that initialises the buffer state by setting it to empty. \<close>
 
 abbreviation Init :: act_buffer where
-"Init \<equiv> buff := []"
+"Init \<equiv> buff :=\<^sub>C []"
 
 text \<open> We define the main body of behaviour for the buffer as an abbreviation. We can either
   input a value and then place it into the buffer, or else, provided that the buffer is non-empty,
   we can output a value presently in the buffer. \<close>
 
+term OutputCSP
+
+utp_lift_notation chan_apply (1)
+
 abbreviation DoBuff :: act_buffer where
 "DoBuff \<equiv> (inp?(val) ;; buff := buff @ [val]
-           \<box> #buff > 0 && outp!(hd(buff)) ;; buff := tl(buff))"
+           \<box> (length(&buff) > 0) && outp!(hd(buff)) ;; buff := tl(buff))"
 
 text \<open> The main action of the buffer first initialises the single state variable $buff$, and
   enters a recursive loop where it does \emph{DoBuff} over and over. \<close>
@@ -56,20 +60,20 @@ lemma Init_contract:
   "Init = \<^bold>R\<^sub>s(true\<^sub>r \<turnstile> false \<diamondop> \<Phi>(true,[&buff \<mapsto>\<^sub>s []],\<langle>\<rangle>))"
   by (rdes_simp)
 
-term "[&buff \<mapsto>\<^sub>s buff @ [\<guillemotleft>x\<guillemotright>]]"
+term chan_apply
 
 lemma DoBuff_contract:
   "DoBuff = \<^bold>R\<^sub>s (true\<^sub>r \<turnstile>
-                \<E>(true,\<langle>\<rangle>, (\<Sqinter> x \<bullet> {(inp\<cdot>\<guillemotleft>x\<guillemotright>)\<^sub>u}\<^sub>u) \<union>\<^sub>u ({(outp\<cdot>head\<^sub>u(&buff))\<^sub>u}\<^sub>u \<triangleleft> 0 <\<^sub>u #\<^sub>u(&buff) \<triangleright> {}\<^sub>u)) \<diamondop>
+                \<E>(true,\<langle>\<rangle>, (\<Sqinter> x \<bullet> {(inp\<cdot>\<guillemotleft>x\<guillemotright>)\<^sub>u}\<^sub>u) \<union>\<^sub>u ({(outp\<cdot>(hd(&buff)))\<^sub>u}\<^sub>u \<triangleleft> 0 <\<^sub>u #\<^sub>u(&buff) \<triangleright> {}\<^sub>u)) \<diamondop>
                 ((\<Sqinter> x \<bullet> \<Phi>(true,[&buff \<mapsto>\<^sub>s buff @ [\<guillemotleft>x\<guillemotright>], val \<mapsto>\<^sub>s \<guillemotleft>x\<guillemotright>],\<langle>(inp\<cdot>\<guillemotleft>x\<guillemotright>)\<^sub>u\<rangle>)) \<or>
-                 \<Phi>(0 <\<^sub>u #\<^sub>u(&buff), [&buff \<mapsto>\<^sub>s tl(buff)], \<langle>(outp\<cdot>head\<^sub>u(&buff))\<^sub>u\<rangle>)))"
+                 \<Phi>(0 <\<^sub>u #\<^sub>u(&buff), [&buff \<mapsto>\<^sub>s tl(buff)], \<langle>(outp\<cdot>(hd(&buff)))\<^sub>u\<rangle>)))"
   by (rdes_eq)
 
 lemma Buffer_contract:
   "Buffer = \<^bold>R\<^sub>s(true\<^sub>r \<turnstile> \<Phi>(true,[&buff \<mapsto>\<^sub>s []],\<langle>\<rangle>) ;;
                        ((\<Sqinter> x \<bullet> \<Phi>(true, [&buff \<mapsto>\<^sub>s buff @ [\<guillemotleft>x\<guillemotright>], val \<mapsto>\<^sub>s \<guillemotleft>x\<guillemotright>], \<langle>(inp\<cdot>\<guillemotleft>x\<guillemotright>)\<^sub>u\<rangle>)) \<or>
-                        \<Phi>(0 <\<^sub>u #\<^sub>u(&buff), [&buff \<mapsto>\<^sub>s tl(buff)], \<langle>(outp\<cdot>head\<^sub>u(&buff))\<^sub>u\<rangle>))\<^sup>\<star>\<^sup>c ;;
-                        \<E>(true,\<langle>\<rangle>, (\<Sqinter> x \<bullet> {(inp\<cdot>\<guillemotleft>x\<guillemotright>)\<^sub>u}\<^sub>u) \<union>\<^sub>u ({(outp\<cdot>head\<^sub>u(&buff))\<^sub>u}\<^sub>u \<triangleleft> 0 <\<^sub>u #\<^sub>u(&buff) \<triangleright> {}\<^sub>u)) \<diamondop>
+                        \<Phi>(0 <\<^sub>u #\<^sub>u(&buff), [&buff \<mapsto>\<^sub>s tl(buff)], \<langle>(outp\<cdot>hd(&buff))\<^sub>u\<rangle>))\<^sup>\<star>\<^sup>c ;;
+                        \<E>(true,\<langle>\<rangle>, (\<Sqinter> x \<bullet> {(inp\<cdot>\<guillemotleft>x\<guillemotright>)\<^sub>u}\<^sub>u) \<union>\<^sub>u ({(outp\<cdot>hd(&buff))\<^sub>u}\<^sub>u \<triangleleft> 0 <\<^sub>u #\<^sub>u(&buff) \<triangleright> {}\<^sub>u)) \<diamondop>
                        false)"
   unfolding Buffer_def DoBuff_contract by (rdes_simp)
 
@@ -81,7 +85,7 @@ abbreviation "inps t \<equiv> [x. inp x \<leftarrow> t]"
 abbreviation "outps t \<equiv> [x. outp x \<leftarrow> t]"
 
 lemma P1_lemma:
-  "[true \<turnstile> (outps(\<guillemotleft>trace\<guillemotright>) \<le> (buff @ inps(\<guillemotleft>trace\<guillemotright>))) | true]\<^sub>C \<sqsubseteq> while\<^sub>C true do DoBuff od"
+  "[true \<turnstile> U(outps(\<guillemotleft>trace\<guillemotright>) \<le> (buff @ inps(\<guillemotleft>trace\<guillemotright>))) | true]\<^sub>C \<sqsubseteq> while\<^sub>C true do DoBuff od"
   apply (rdes_refine_split)
     apply (simp_all add: rpred closure usubst)
   apply (rule conjI)
@@ -99,17 +103,17 @@ lemma P1_lemma:
     apply (smt Prefix_Order.Cons_prefix_Cons append.left_neutral append_Cons ch_buffer.simps(6) concat_map_maps hd_Cons_tl less_eq_list_def maps_simps(1) prefix_code(2))
 done 
 
-lemma P1: "[true \<turnstile> outps(\<guillemotleft>trace\<guillemotright>) \<le> inps(\<guillemotleft>trace\<guillemotright>) | true]\<^sub>C \<sqsubseteq> Buffer"
+lemma P1: "[true \<turnstile> U(outps(\<guillemotleft>trace\<guillemotright>) \<le> inps(\<guillemotleft>trace\<guillemotright>)) | true]\<^sub>C \<sqsubseteq> Buffer"
 proof -
-  have "[true \<turnstile> outps(\<guillemotleft>trace\<guillemotright>) \<le> inps(\<guillemotleft>trace\<guillemotright>) | true]\<^sub>C
+  have "[true \<turnstile> U(outps(\<guillemotleft>trace\<guillemotright>) \<le> inps(\<guillemotleft>trace\<guillemotright>)) | true]\<^sub>C
         \<sqsubseteq>
-        Init ;; [true \<turnstile> outps(\<guillemotleft>trace\<guillemotright>) \<le> inps(\<guillemotleft>trace\<guillemotright>) | true]\<^sub>C"
+        Init ;; [true \<turnstile> U(outps(\<guillemotleft>trace\<guillemotright>) \<le> inps(\<guillemotleft>trace\<guillemotright>)) | true]\<^sub>C"
     by (rdes_refine)
-  moreover have "Init ;; [true \<turnstile> outps(\<guillemotleft>trace\<guillemotright>) \<le> inps(\<guillemotleft>trace\<guillemotright>) | true]\<^sub>C 
+  moreover have "Init ;; [true \<turnstile> U(outps(\<guillemotleft>trace\<guillemotright>) \<le> inps(\<guillemotleft>trace\<guillemotright>)) | true]\<^sub>C 
                  \<sqsubseteq>
-                 Init ;; [true \<turnstile> outps(\<guillemotleft>trace\<guillemotright>) \<le> (buff @ inps(\<guillemotleft>trace\<guillemotright>)) | true]\<^sub>C"
+                 Init ;; [true \<turnstile> U(outps(\<guillemotleft>trace\<guillemotright>) \<le> (buff @ inps(\<guillemotleft>trace\<guillemotright>))) | true]\<^sub>C"
     by (rdes_refine)
-  moreover have "Init ;; [true \<turnstile> outps(\<guillemotleft>trace\<guillemotright>) \<le> (buff @ inps(\<guillemotleft>trace\<guillemotright>)) | true]\<^sub>C
+  moreover have "Init ;; [true \<turnstile> U(outps(\<guillemotleft>trace\<guillemotright>) \<le> (buff @ inps(\<guillemotleft>trace\<guillemotright>))) | true]\<^sub>C
                  \<sqsubseteq>
                  Buffer"
     by (simp add: Buffer_def P1_lemma urel_dioid.mult_isol)
