utp/utp_state_parser.thy
@@ -1,7 +1,7 @@
 section \<open> State Variable Declaration Parser \<close>
 
 theory utp_state_parser
-  imports "utp_rel"
+  imports "utp_blocks"
 begin
 
 text \<open> This theory sets up a parser for state blocks, as an alternative way of providing lenses to
@@ -27,12 +27,13 @@ syntax
   "_pairT" :: "type \<Rightarrow> type \<Rightarrow> type" ("PAIRTYPE'(_, _')")
   "_state_type" :: "pttrn \<Rightarrow> type"
   "_state_tuple" :: "type \<Rightarrow> pttrn \<Rightarrow> logic"
-  "_state_lenses" :: "pttrn \<Rightarrow> logic"
-  "_state_decl" :: "pttrn \<Rightarrow> logic \<Rightarrow> logic" ("LOCAL _ \<bullet> _" [0, 10] 10) 
+  "_state_lenses" :: "pttrn \<Rightarrow> logic \<Rightarrow> logic"
+  "_state_decl" :: "pttrn \<Rightarrow> logic \<Rightarrow> logic" ("alpha _ \<bullet> _" [0, 10] 10) 
+  "_state_decl_in" :: "pttrn \<Rightarrow> logic \<Rightarrow> logic \<Rightarrow> logic" ("alpha _ in _ \<bullet> _" [0, 0, 10] 10)
 
 translations
   (type) "PAIRTYPE('a, 'b)" => (type) "'a \<times> 'b"
-  (type) "LENSTYPE('a, 'b)" => (type) "'a \<Longrightarrow> 'b"
+  (type) "LENSTYPE('a, 'b)" => (type) "'a \<Longrightarrow> _"
 
   "_state_type (_constrain x t)" => "t"
   "_state_type (CONST Pair (_constrain x t) vs)" => "_pairT t (_state_type vs)"
@@ -41,41 +42,64 @@ translations
   "_state_tuple st (CONST Pair (_constrain x t) vs)" =>
     "CONST Product_Type.Pair (_constrain x (_lensT t st)) (_state_tuple st vs)"
 
+  "_state_decl_in vs loc P" =>
+    "CONST state_block (_abs (_state_tuple (_state_type vs) vs) P) (_state_lenses vs loc)"
+
   "_state_decl vs P" =>
-    "CONST state_block (_abs (_state_tuple (_state_type vs) vs) P) (_state_lenses vs)"
+    "CONST state_block (_abs (_state_tuple (_state_type vs) vs) P) (_state_lenses vs 1\<^sub>L)"
   "_state_decl vs P" <= "CONST state_block (_abs vs P) k"
 
-parse_translation {*
+ML \<open>
+
+ \<close>
+
+parse_translation \<open>
   let
-    open HOLogic;
-    val lens_comp = Const (@{const_syntax "lens_comp"}, dummyT);
-    val fst_lens = Const (@{const_syntax "fst_lens"}, dummyT);
+    open HOLogic; open Syntax;
+    fun lensT s t = Type (@{type_name lens_ext}, [s, t, HOLogic.unitT]);
+    fun lens_comp a b c = Const (@{const_syntax "lens_comp"}, lensT a b --> lensT b c --> lensT a c);
+    fun fst_lens t = Const (@{const_syntax "fst_lens"}, Type (@{type_name lens_ext}, [t, dummyT, unitT]));
     val snd_lens = Const (@{const_syntax "snd_lens"}, dummyT);
-    val id_lens = Const (@{const_syntax "id_lens"}, dummyT);
+    fun id_lens t = Const (@{const_syntax "id_lens"},Type (@{type_name lens_ext}, [t, dummyT, unitT]));
+    fun lens_syn_typ t = const @{type_syntax lens_ext} $ t $ const @{type_syntax dummy} $ const @{type_syntax unit};
+    fun constrain t ty = const @{syntax_const "_constrain"} $ t $ ty;
+
+    (* Construct a tuple of n lenses, whose source type is product of the types in ts, and each lens
+       has an element of the type: prod_lens [t0, t1 ... ] 1 : t1 ==> t0 * t1 * ... *)
+    fun prod_lens ts i = 
+      let open Syntax; open Library; fun lens_compf (x, y) = const @{const_name lens_comp} $ x $ y in
+      if (length ts = 1) 
+      then Const (@{const_name id_lens}, lensT (nth ts i) (nth ts i))
+      else if (length ts = i + 1) 
+      then foldl lens_compf (Const (@{const_name "snd_lens"}, lensT (nth ts i) dummyT), replicate (i-1) (const @{const_name "snd_lens"}))
+      else foldl lens_compf (Const (@{const_name "fst_lens"}, lensT (nth ts i) dummyT), replicate i (const @{const_name "snd_lens"}))
+      end;
+
     (* Construct a tuple of lenses for each of the possible locally declared variables *)
-    fun 
-      state_lenses n st = 
-        if (n = 1) 
-          then st
-          else pair_const dummyT dummyT $ (lens_comp $ fst_lens $ st) $ (state_lenses (n - 1) (lens_comp $ snd_lens $ st));
+    fun state_lenses ts sty st = 
+      foldr1 (fn (x, y) => pair_const dummyT dummyT $ x $ y) (map (fn i => lens_comp dummyT sty dummyT $ prod_lens ts i $ st) (upto (0, length ts - 1)));
+
     fun
       (* Add up the number of variable declarations in the tuple *)
       var_decl_num (Const (@{const_syntax "Product_Type.Pair"},_) $ _ $ vs) = var_decl_num vs + 1 |
       var_decl_num _ = 1;
 
-    
-    fun state_lens ctx [vs] = state_lenses (var_decl_num vs) id_lens ;
+    fun
+      var_decl_typs (Const (@{const_syntax "Product_Type.Pair"},_) $ (Const ("_constrain", _) $ _ $ typ) $ vs) = Syntax_Phases.decode_typ typ :: var_decl_typs vs |
+      var_decl_typs (Const ("_constrain", _) $ _ $ typ) = [Syntax_Phases.decode_typ typ] |
+      var_decl_typs _ = [];
+
+    fun state_lens ctx [vs, loc] = (state_lenses (var_decl_typs vs) (mk_tupleT (var_decl_typs vs)) loc);
   in
   [("_state_lenses", state_lens)]
   end
-*}
+\<close>
 
 subsection \<open> Examples \<close>
 
-term  "LOCAL (x::int, y::real, z::int) \<bullet> x := (&x + &z)"
+term "alpha (x::int, y::real, z::int) \<bullet> y := &x + &z"
 
-lemma "LOCAL p \<bullet> II = II"
+lemma "alpha p \<bullet> II = II"
   by (rel_auto)
-
 
 end
