utp/utp_wp.thy
@@ -12,6 +12,8 @@ consts
 
 no_utp_lift uwp
 
+utp_lift_notation uwp (1)
+
 syntax
   "_uwp" :: "logic \<Rightarrow> uexp \<Rightarrow> logic" (infix "wp" 60)
 
